2x1
ㅁ
ㅁ
(1x2, 1)
= 1

2x2
ㅁㅁ
ㅁㅁ
(2x1, 2)
(1x2, 2)
= 2

2x3
ㅁㅁㅁ
ㅁㅁㅁ
(1x2, 3)
(1x2, 1) + (2x1, 2)
(2x1, 2) + (1x2, 1)
= 3

2x4
ㅁㅁㅁㅁ
ㅁㅁㅁㅁ
(1x2, 4)
(1x2, 2) + (2x1, 2)
(1x2, 1) + (2x1, 2) + (1x2, 1)
(2x1, 2) + (1x2, 2)
(2x1, 4)
= 5

2x5
ㅁㅁㅁㅁㅁ
ㅁㅁㅁㅁㅁ
(1x2, 5)
(1x2, 4) -> X
(1x2, 3) + (2x1, 2)
(1x2, 2) + (2x1, 2) + (1x2, 1)
(1x2, 1) + (2x1, 2) + (1x2, 2)
(1x2, 1) + (2x1, 4)
(2x1, 5) -> X
(2x1, 4) + (1x2, 1)
(2x1, 3) -> X
(2x1, 2) + (1x2, 1) + (2x1, 2)
(2x1, 2) + (1x2, 3)
= 8

2x6 = 13

2x7 = 21

2x8 = 34

2x9 = 55
